
\documentclass[12pt]{article}
 
\usepackage[margin=1in]{geometry} 
\usepackage{amsmath,amsthm,amssymb,scrextend}
\usepackage{fancyhdr}
\pagestyle{fancy}
\DeclareMathOperator{\rng}{Rng}
\DeclareMathOperator{\dom}{Dom}
\newcommand{\R}{\mathbb R}
\newcommand{\cont}{\subseteq}
\newcommand{\N}{\mathbb N}
\newcommand{\Z}{\mathbb Z}
\usepackage{tikz}
\usepackage{pgfplots}
\usepackage{amsmath}
\usepackage[mathscr]{euscript}
\let\euscr\mathscr \let\mathscr\relax% just so we can load this and rsfs
\usepackage[scr]{rsfso}
\usepackage{amsthm}
\usepackage{amssymb}
\usepackage{multicol}
%\usepackage{ngerman}
\usepackage[colorlinks=true, pdfstartview=FitV, linkcolor=blue,
citecolor=blue, urlcolor=blue]{hyperref}

\DeclareMathOperator{\arcsec}{arcsec}
\DeclareMathOperator{\arccot}{arccot}
\DeclareMathOperator{\arccsc}{arccsc}
\newcommand{\ddx}{\frac{d}{dx}}
\newcommand{\dfdx}{\frac{df}{dx}}
\newcommand{\ddxp}[1]{\frac{d}{dx}\left( #1 \right)}
\newcommand{\dydx}{\frac{dy}{dx}}
\let\ds\displaystyle
\newcommand{\intx}[1]{\int #1 \, dx}
\newcommand{\intt}[1]{\int #1 \, dt}
\newcommand{\defint}[3]{\int_{#1}^{#2} #3 \, dx}
\newcommand{\imp}{\Rightarrow}
\newcommand{\un}{\cup}
\newcommand{\inter}{\cap}
\newcommand{\ps}{\mathscr{P}}
\newcommand{\set}[1]{\left\{ #1 \right\}}
\newtheorem*{sol}{Solution}
\newtheorem*{claim}{Claim}
\newtheorem{problem}{Problem}
\begin{document}
 

\lhead{Formal Logic Sheet 2}
\chead{Robert Feldhans, Sebastian Mueller}
\rhead{\today}


\section*{Exercise 5:  (Laws of Logic)}

\subsection*{1.}
$F \land (F \lor G) \equiv F$\\
$\Leftrightarrow (F \land F) \lor (F \land G) \equiv F$ \hspace*{2cm} see part 2\\
$\Leftrightarrow F \lor (F \land G) \equiv F$\\\\
So the truth table for both formulae looks like this:\\\\
\begin{tabular}{  l | l | l }
	F G & $F \lor G$ & $F \land (F \lor G) $  \\ \hline
	0 0 & 0 & 0  \\
	0 1 & 1 & 0  \\
	1 0 & 1 & 1  \\
	1 1 & 1 & 1  \\
\end{tabular}

\subsection*{2.}
$F \land (G \lor H) \equiv (F \land G) \lor (F \land H)$\\
\begin{tabular}{  l | l | l | l | l | l}
	F G H & $G \lor H$ & $F \land (G \lor H) $ & $F \land G$ & $F \land H$ & $(F \land G) \lor (F \land H)$ \\ \hline
	0 0 0 & 0 & 0 & 0 & 0 & 0\\
	0 0 1 & 1 & 0 & 0 & 0 & 0\\
	0 1 0 & 1 & 0 & 0 & 0 & 0\\
	0 1 1 & 1 & 0 & 0 & 0 & 0\\
	1 0 0 & 0 & 0 & 0 & 0 & 0\\
	1 0 1 & 1 & 1 & 0 & 1 & 1\\
	1 1 0 & 1 & 1 & 1 & 0 & 1\\
	1 1 1 & 1 & 1 & 1 & 1 & 1\\
\end{tabular}\\\\\\
$F \lor (G \land H) \equiv (F \lor G) \land (F \lor H)$\\
\begin{tabular}{  l | l | l | l | l | l}
	F G H & $G \land H$ & $F \lor (G \land H) $ & $F \lor G$ & $F \lor H$ & $(F \lor G) \land (F \lor H)$ \\ \hline
	0 0 0 & 0 & 0 & 0 & 0 & 0\\
	0 0 1 & 0 & 0 & 0 & 1 & 0\\
	0 1 0 & 0 & 0 & 1 & 0 & 0\\
	0 1 1 & 1 & 1 & 1 & 1 & 1\\
	1 0 0 & 0 & 1 & 1 & 1 & 1\\
	1 0 1 & 0 & 1 & 1 & 1 & 1\\
	1 1 0 & 0 & 1 & 1 & 1 & 1\\
	1 1 1 & 1 & 1 & 1 & 1 & 1\\
\end{tabular}

\subsection*{3.}
$\neg (F \land G) \equiv \neg F \lor \neg G$\\
\begin{tabular}{  l | l | l }
	F G & $F \land G$ & $\neg F \lor \neg G$  \\ \hline
	0 0 & 0 & 1  \\
	0 1 & 0 & 1  \\
	1 0 & 0 & 1  \\
	1 1 & 1 & 0  \\
\end{tabular}\\\\
$\neg (F \lor G) \equiv \neg F \land \neg G$\\
\begin{tabular}{  l | l | l }
	F G & $F \lor G$ & $\neg F \land \neg G$  \\ \hline
	0 0 & 0 & 1 \\
	0 1 & 1 & 0  \\
	1 0 & 1 & 0  \\
	1 1 & 1 & 0  \\
\end{tabular}

\section*{Exercise 6: (Two proofs)}

Show $F_1 = (A \lor \lnot (B \land A)) \land (C \lor (D \lor C)) = C \lor D = F_2$\\ \\
(a) by truth table\\
\begin{tabular}{  l | l | l | l | l | l | l  }
	A B C D & $\lnot (B \land A)$ & $A \lor \lnot (B \land A) = G_1$ & $D \lor C$ & $C \lor (D \lor C) = G_2$ & $F_1 = G_1 \land G_2$ & $F_2 = C \lor D$ \\ \hline
	0 0 0 0 & 1 &1 &0 &0 &0 &0  \\
	0 0 0 1 & 1 &1 &1 &1 &1 &1  \\
	0 0 1 0 & 1 &1 &1 &1 &1 &1  \\
	0 0 1 1 & 1 &1 &1 &1 &1 &1  \\
	0 1 0 0 & 1 &1 &0 &0 &0 &0  \\
	0 1 0 1 & 1 &1 &1 &1 &1 &1  \\
	0 1 1 0 & 1 &1 &1 &1 &1 &1  \\
	0 1 1 1 & 1 &1 &1 &1 &1 &1  \\
	1 0 0 0 & 1 &1 &0 &0 &0 &0  \\
	1 0 0 1 & 1 &1 &1 &1 &1 &1  \\
	1 0 1 0 & 1 &1 &1 &1 &1 &1  \\
	1 0 1 1 & 1 &1 &1 &1 &1 &1  \\
	1 1 0 0 & 0 &1 &0 &0 &0 &0  \\
	1 1 0 1 & 0 &1 &1 &1 &1 &1  \\
	1 1 1 0 & 0 &1 &1 &1 &1 &1  \\
	1 1 1 1 & 0 &1 &1 &1 &1 &1  \\
	
\end{tabular}
\\ \\
(b) by transformation \\
	$F_1 = (A \lor \lnot (B \land A)) \land (C \lor (D \lor C)) \\
	\overset{de Morgan}{=} ( A \lor ( \lnot B \lor \lnot A)) \land (C \lor (D \lor C)) \\
	\overset{Assoc.}{=} ( A \lor \lnot B \lor \lnot A) \land (C \lor D \lor C) \\
	\overset{Idemp.}{=} \underset{Tautology}{( A \lor \lnot B \lor \lnot A)} \land (C \lor D) \\
	 = C \lor D \ = F_2$ 

\section*{Exercise 7: (CNF and DNF)}
$ F = (\lnot A \implies B) \lor ((A \lor \lnot C) \Leftrightarrow B)\\
 = (\lnot\lnot A \lor B) \lor (((A \land \lnot C)\land B) \lor (\lnot(A\land \lnot C)\land \lnot B)) $\\ \\ 
1. \\
 Replace Double negations\\
 $\Leftrightarrow (A \lor B) \lor (((A \land \lnot C)\land B) \lor (\lnot(A\land \lnot C)\land \lnot B))$\\ \\
 Apply De Morgan's rules\\
 $\Leftrightarrow A \lor B \lor (A \land \lnot C \land B) \lor ((\lnot A \lor C) \land \lnot B)$\\ \\
2. \\
DNF\\
$\Leftrightarrow A \lor B \lor (A \land \lnot C \land B) \lor  (\lnot A \land B) \lor (C \land \lnot B)$ \\ \\
CNF\\
 $\Leftrightarrow A \lor B \lor 
 (((A \land \lnot C \land B) \lor (\lnot A \lor C)) \land (\lnot B \lor (A \land \lnot C \land B)))$\\
 $\Leftrightarrow A \lor B \lor 
 (((\underset{Tautology}{A \lor (\lnot A \lor C)}) \land (B \lor (\lnot A \lor C) \land \underset{Tautology}{(\lnot C \lor (\lnot A \lor C))} \land ((\lnot B \lor A) \land (\lnot B \lor C) \land (\underset{Tautology}{\lnot B \lor B})))$\\
 $\Leftrightarrow A \lor B \lor 
 ((B \lor \lnot A \lor C) \land (\lnot B \lor A) \land (\lnot B \lor C))$\\
$\Leftrightarrow A \lor ((B \lor B \lor \lnot A \lor C) \land (\underset{Tautology}{B \lor \lnot B \lor A)} \land (\underset{Tautology}{B \lor \lnot B \lor C}))$\\
$\Leftrightarrow \underset{Tautology}{A \lor (B \lor B \lor \lnot A \lor C)} = 1$\\ \\

\section*{Exercise 8: (Switch and and or)}
No solution.

%ANARCHY
\end{document}