
\documentclass[12pt]{article}
 
\usepackage[margin=1in]{geometry} 
\usepackage{amsmath,amsthm,amssymb,scrextend}
\usepackage{fancyhdr}
\pagestyle{fancy}
\DeclareMathOperator{\rng}{Rng}
\DeclareMathOperator{\dom}{Dom}
\newcommand{\R}{\mathbb R}
\newcommand{\cont}{\subseteq}
\newcommand{\N}{\mathbb N}
\newcommand{\Z}{\mathbb Z}
\usepackage{tikz}
\usepackage{pgfplots}
\usepackage{amsmath}
\usepackage[mathscr]{euscript}
\let\euscr\mathscr \let\mathscr\relax% just so we can load this and rsfs
\usepackage[scr]{rsfso}
\usepackage{amsthm}
\usepackage{amssymb}
\usepackage{multicol}
%\usepackage{ngerman}
\usepackage[colorlinks=true, pdfstartview=FitV, linkcolor=blue,
citecolor=blue, urlcolor=blue]{hyperref}

\DeclareMathOperator{\arcsec}{arcsec}
\DeclareMathOperator{\arccot}{arccot}
\DeclareMathOperator{\arccsc}{arccsc}
\newcommand{\ddx}{\frac{d}{dx}}
\newcommand{\dfdx}{\frac{df}{dx}}
\newcommand{\ddxp}[1]{\frac{d}{dx}\left( #1 \right)}
\newcommand{\dydx}{\frac{dy}{dx}}
\let\ds\displaystyle
\newcommand{\intx}[1]{\int #1 \, dx}
\newcommand{\intt}[1]{\int #1 \, dt}
\newcommand{\defint}[3]{\int_{#1}^{#2} #3 \, dx}
\newcommand{\imp}{\Rightarrow}
\newcommand{\un}{\cup}
\newcommand{\inter}{\cap}
\newcommand{\ps}{\mathscr{P}}
\newcommand{\set}[1]{\left\{ #1 \right\}}
\newtheorem*{sol}{Solution}
\newtheorem*{claim}{Claim}
\newtheorem{problem}{Problem}
\begin{document}
 

\lhead{Formal Logic Sheet 3}
\chead{Robert Feldhans, Sebastian Mueller}
\rhead{\today}


\section*{Exercise 9:  (Horn formula algorithm)}

First, we write the formula in the implication-form, so \\
$F = (\neg A \lor \neg B \lor \neg D) \land \neg E \land (\neg C \lor A) \land C \land B \land (\neg G \lor D) \land G$\\
becomes:\\
$F = (A \land B \land D \Rightarrow 0) \land (0 \Rightarrow E) \land (C \Rightarrow A) \land (1 \Rightarrow C) \land (1 \Rightarrow B) \land (G \Rightarrow D) \land (1 \Rightarrow G)$\\\\
Then we start marking all literals of the form $(1 \Rightarrow X)$:\\
$F = (A \land B \land D \Rightarrow 0) \land (0 \Rightarrow E) \land (C \Rightarrow A) \land \underline{(1 \Rightarrow C)} \land \underline{(1 \Rightarrow B)} \land (G \Rightarrow D) \land \underline{(1 \Rightarrow G)}$\\\\
Now we start with the loop part of the algorithm: \\
$F = (A \land B \land D \Rightarrow 0) \land (0 \Rightarrow E) \land \underline{(C \Rightarrow A)} \land \underline{(1 \Rightarrow C)} \land \underline{(1 \Rightarrow B)} \land (G \Rightarrow D) \land \underline{(1 \Rightarrow G)}$\\\\
$F = (A \land B \land D \Rightarrow 0) \land (0 \Rightarrow E) \land \underline{(C \Rightarrow A)} \land \underline{(1 \Rightarrow C)} \land \underline{(1 \Rightarrow B)} \land \underline{(G \Rightarrow D)} \land \underline{(1 \Rightarrow G)}$\\\\
In the next step we would mark the $(A \land B \land D \Rightarrow 0)$ literal, but it implies 0, so the formula is non satisfiable.


\section*{Exercise 10: (Not a Horn formula)}

\subsection*{a.}

\subsection*{b}

\section*{Exercise 11:  ($\neg$ and $\Rightarrow$ suffice, but $\lor$, $\land$ and $\Rightarrow$ donâ€™t)}

\subsection*{a.}

\subsection*{b}

\section*{Exercise 12: (Infinitely many formulas)}

%ANARCHY
\end{document}